src/lowparse/LowParseExample4.Aux.fsti
@@ -1,4 +1,4 @@
-module LowParseExample4
+module LowParseExample4.Aux
 
 module LPC = LowParse.Spec.Combinators
 module LPI = LowParse.Low.Int
@@ -61,21 +61,3 @@ val parse_t_intro
     LP.exactly_contains_valid_data h parse_t b lo ({ inner = l; last = r; }) hi
   ))
   [SMTPat (LP.exactly_contains_valid_data h (parse_inner `LPC.nondep_then` LPI.parse_u32) b lo x hi)]
-
-(*
-#set-options "--z3rlimit 32"
-
-let main: Int32.t -> FStar.Buffer.buffer (FStar.Buffer.buffer C.char) ->
-   HST.Stack C.exit_code (fun _ -> true) (fun _ _ _ -> true)
-=
-  fun _ _ ->
-  HST.push_frame ();
-  let b : LP.buffer8 = B.alloca 0uy 8ul in
-//  assert (B.len b == 8ul);
-  LPI.serialize32_u16 b 0ul 18us;
-  LPI.serialize32_u16 b 2ul 42us;
-  LPI.serialize32_u32 b 4ul 1729ul;
-  let h = HST.get () in
-  assert (LP.exactly_contains_valid_data h parse_t b 0ul ({ inner = ({ left = 18us; right = 42us; }); last = 1729ul;}) 8ul);
-  HST.pop_frame ();
-  C.EXIT_SUCCESS
